---
layout: post
title: "test"
date: 2005-12-18 23:26:38 +0800
comments: true
categories:
mathjax: true
---

When $$a \ne 0$$, there are two solutions to $$ax^2 + bx + c = 0$$ and they are

$$x_1 = {-b + \sqrt{b^2-4ac} \over 2a}$$
$$x_2 = {-b - \sqrt{b^2-4ac} \over 2a} \notag$$

$$ \begin{align*} y = y(x,t) &= A e^{i\theta} \\ &= A (\cos \theta + i \sin \theta) \\ &= A (\cos(kx - \omega t) + i \sin(kx - \omega t)) \\ &= A\cos \frac{2\pi}{\lambda} (x - v t) + i A\sin \frac{2\pi}{\lambda} (x - v t) \end{align*} $$
